Leanduction/Examples.lean
@@ -2,22 +2,17 @@ import Leanduction.SparseParametricity
 import Leanduction.SparseRecursor
 
 inductive Weird (α : Type) : Nat → Type where
-  | node : (Int → Option (Int → List (Int → Weird α 0))) → Weird α 0
+  | node n : (Int → Option (Int → List (Int → Weird α 0))) → Weird α n
 
--- #gen_sparse_rec Weird
-
-set_option trace.Sparse.Recursor true
+#gen_sparse_rec -indElim Weird as Weird.s
 
 inductive Tree (α : Type) :  Type where
   | node : α → (a : List (Tree α)) → Tree α
 
--- #gen_sparse Tree
 #gen_sparse_rec Tree
 
 def Tree.map (f : α → β) : Tree α → Tree β
   | node x children => .node (f x) (children.map (Tree.map f))
-
-#print List.All
 
 example (t : Tree α) : t.map id = t := by
   induction t with
