Leanduction/Util.lean
@@ -1,0 +1,13 @@
+import Lean
+
+open Lean Elab Meta
+
+def checkConstant (name : Name): MetaM Unit := do
+  if (← getEnv).contains name then
+    throwError "`{.ofConstName name true}` has already been declared"
+
+/-- Transforms expressions of shape `fun x => f x` to `f` when x doesn't appear in `f`, useful to generate better looking recursors-/
+partial def Lean.Expr.tryEtaReduce (e: Expr): Expr :=
+  match e with
+    | .lam _ _ (.app f (.bvar 0)) _ => if f.hasLooseBVar 0 then e else f |>.lowerLooseBVars 0 1 |>.tryEtaReduce
+    | _ => e
